wip
squash! wip

wrapper.v
@@ -34,4 +34,141 @@ Definition wrapper : full_contract false parameter_ty None storage_ty :=
   DIP1 {SWAP; PAIR};
   PAIR
 }.
+
+Local Definition exec
+(A : instruction_seq None false (pair bytes bytes ::: [::])
+                 (pair (list operation) bytes ::: [::]))
+: instruction_seq (Some (parameter_ty, None)) false
+                  (pair (pair bytes bytes) (option (pair address (pair syntax_type.string syntax_type.string))) ::: [::])
+              (pair (list operation) storage_ty ::: [::]) :=
+{
+  UNPAIR;
+  LAMBDA (pair bytes bytes) (pair (list operation) bytes) A;
+  SWAP;
+  EXEC;
+  UNPAIR;
+  DIP1 {PAIR; PUSH _ (Instruction false A); PAIR};
+  PAIR
+}.
+Import Notations.
+
+Lemma bind_id T (A1 : M (T * Datatypes.unit)) :
+  bind A1 (fun '(x, tt) => Return (x, tt)) = A1.
+Proof. by case: A1 => []//[]// + []. Qed.
+
+Definition exec_correct_success
+(arg : data bytes)
+(wstore : data bytes)
+(avt_id : data (option (pair address (pair syntax_type.string syntax_type.string))))
+(env : @proto_env (Some (parameter_ty, None)))
+(A : instruction_seq None false (pair bytes bytes ::: [::])
+                 (pair (list operation) bytes ::: [::]))
+fuel returned_operations new_storage :
+  4 <= fuel ->
+  eval_seq (no_self env) A fuel (arg, wstore, tt) = Return (returned_operations, new_storage, tt) ->
+  eval_seq env (exec A) fuel.+1 (arg, wstore, avt_id, tt) =
+  Return (returned_operations,
+          ((existT _ false A : data (lambda (pair bytes bytes)
+                                            (pair (list operation) bytes))),
+           (new_storage, avt_id)), tt).
+Proof.
+  move=> Hfuel.
+  have<-: 3 + (fuel - 3) = fuel by rewrite addnC subnK // (ltn_trans _ Hfuel).
+  by rewrite /eval_seq /= => ->.
+Qed.
+
+Definition exec_correct_fail
+(arg : data bytes)
+(wstore : data bytes)
+(avt_id : data (option (pair address (pair syntax_type.string syntax_type.string))))
+(env : @proto_env (Some (parameter_ty, None)))
+(A : instruction_seq None false (pair bytes bytes ::: [::])
+                 (pair (list operation) bytes ::: [::]))
+fuel e :
+  4 <= fuel ->
+  eval_seq (no_self env) A fuel (arg, wstore, tt) = Failed _ e ->
+  eval_seq env (exec A) fuel.+1 (arg, wstore, avt_id, tt) = Failed _ e.
+Proof.
+  move=> Hfuel.
+  have<-: 3 + (fuel - 3) = fuel by rewrite addnC subnK // (ltn_trans _ Hfuel).
+  by rewrite /eval_seq /= => ->.
+Qed.
+
+Lemma wrapper_correct_success
+(arg : data bytes)
+(wstore : data bytes)
+(avt_id : data (option (pair address (pair syntax_type.string syntax_type.string))))
+(env : @proto_env (Some (parameter_ty, None)))
+(A : instruction_seq None false (pair bytes bytes ::: [::])
+                 (pair (list operation) bytes ::: [::]))
+(fuel : Datatypes.nat) returned_operations new_storage :
+  4 <= fuel ->
+  eval_seq (no_self env) A fuel (arg, wstore, tt) = Return (returned_operations, new_storage, tt) ->
+  eval_seq env wrapper fuel.+1 (arg, ((existT _ false A : data (lambda (pair bytes bytes)
+                                         (pair (list operation) bytes))), (wstore, avt_id)), tt)
+= Return (returned_operations,
+          ((existT _ false A : data (lambda (pair bytes bytes)
+                                            (pair (list operation) bytes))),
+           (new_storage, avt_id)), tt).
+  rewrite !return_precond !eval_seq_precond_correct => Hfuel.
+  have<-: 4 + (fuel - 4) = fuel by rewrite addnC subnK.
+  move: (eval_seq_precond_eqv _ (no_self env) false _ _ A (4 + (fuel - 4)) (arg, wstore, tt)
+  (fun '(y, tt) =>
+     let (x, _) := y in
+     let (_, y1) := y in
+     (x, (existT (fun tff : Datatypes.bool => instruction_seq None tff (pair (Comparable_type bytes) (Comparable_type bytes) ::: [::]) (pair (list operation) (Comparable_type bytes) ::: [::])) false A, (y1, avt_id)), tt) =
+     (returned_operations, (existT (fun tff : Datatypes.bool => instruction_seq None tff (pair (Comparable_type bytes) (Comparable_type bytes) ::: [::]) (pair (list operation) (Comparable_type bytes) ::: [::])) false A, (new_storage, avt_id)), tt))
+    (eq^~ (returned_operations, new_storage, tt))).
+  rewrite /eval_seq_precond /= => H H0.
+  rewrite H; first by apply H0.
+  case => [] [] a b [].
+  split; by case => -> ->.
+Qed.
+
+Lemma wrapper_correct'
+(arg : data bytes)
+(wstore : data bytes)
+(avt_id : data (option (pair address (pair syntax_type.string syntax_type.string))))
+(env : @proto_env (Some (parameter_ty, None)))
+(A : instruction_seq None false (pair bytes bytes ::: [::])
+                 (pair (list operation) bytes ::: [::]))
+(fuel : Datatypes.nat) :
+  fuel > 10 ->
+  eval_seq (no_self env) A (7 + (fuel - 7)) (arg, wstore, tt)
+= eval_seq (no_self env) A (fuel - 7) (arg, wstore, tt) ->
+  eval_seq env wrapper fuel (arg, ((existT _ false A : data (lambda (pair bytes bytes)
+                                         (pair (list operation) bytes))), (wstore, avt_id)), tt)
+= eval_seq env (exec A) fuel (arg, wstore, avt_id, tt).
+Proof.
+  move=> Hf sA /=.
+  have?: 6 < fuel by apply/(leq_trans _ Hf).
+  have<-: (fuel - 7) + 7 = fuel by rewrite subnK.
+  suff->: 6 + (fuel - 7 + 7) = 4 + ((fuel - 7 + 7) + 2).
+  rewrite /eval_seq /=.
+set X := RHS.
+
+  rewrite /=.
+  rewrite !bind_id.
+  vm_compute.
+
+  simpl.
+  rewrite /wrapper /=.
+  rewrite /=.
+  rewrite addnC.
+  set A1 := (eval _ A _ _).
+  rewrite /= !bind_id; set A2 := (eval _ A _ _).
+  have->: A1 = A2 by subst A1 A2; rewrite sA.
+  have<-: 4 + ((fuel - 7) - 4) = fuel - 7
+   by rewrite addnC subnK // /leq subnBA // subn_eq0 (leq_trans _ Hf).
+  by case: A2 => []//= [][] /=.
+
+
+  Check eval_seq env A.
+LAMBDA _ _ A;; SWAP;;
+EXEC;; UNPAIR;; DIP1 (PUSH _ (Bytes_constant (pack_lambda A)));;
+DIP1 PAIR;; PAIR.
+
+
+Check (instruction None false (lambda (pair bytes bytes) (pair (list operation) bytes))).
+
 End wrapper.
